WIP

Access.v
@@ -8,76 +8,70 @@ From Elo Require Import CoreExt.
 From Elo Require Import AnyTerm.
 From Elo Require Import ValidAddresses.
 
-
 (*
   A term has access to an address if it refers to the address directly or 
   indirectly.
   
   Ignores <spawn> blocks.
 *)
-Reserved Notation " '(' m '|' t ')' 'has_access_to' ad "
-  (at level 90, t custom elo_tm, no associativity).
-Reserved Notation " '(' m '/' t ')' 'has_access_to' ad "
-  (at level 90, no associativity).
-
-Inductive access (m : mem) : addr -> tm -> Prop :=
-  | acc_mem : forall ad ad' T,
+Inductive access (ad : addr) (m : mem) : tm -> Prop :=
+  | acc_mem : forall ad' T,
     ad <> ad' ->
-    (m /  m[ad'].tm) has_access_to ad ->
-    (m | &ad' :: T) has_access_to ad
+    access ad m m[ad'].tm ->
+    access ad m <{&ad' :: T}>
 
-  | acc_ad : forall ad T,
-    (m | &ad :: T) has_access_to ad
+  | acc_ad : forall T,
+    access ad m <{&ad :: T}>
 
-  | acc_new : forall T t ad,
-    (m | t) has_access_to ad ->
-    (m | new T t) has_access_to ad
+  | acc_new : forall T t,
+    access ad m t ->
+    access ad m <{new T t}>
 
-  | acc_load : forall t ad,
-    (m | t) has_access_to ad ->
-    (m | *t) has_access_to ad
+  | acc_load : forall t,
+    access ad m t ->
+    access ad m <{*t}>
 
-  | acc_asg1 : forall t1 t2 ad,
-    (m | t1) has_access_to ad ->
-    (m | t1 = t2) has_access_to ad
+  | acc_asg1 : forall t1 t2,
+    access ad m t1 ->
+    access ad m <{t1 = t2}>
 
-  | acc_asg2 : forall t1 t2 ad,
-    (m | t2) has_access_to ad ->
-    (m | t1 = t2) has_access_to ad
+  | acc_asg2 : forall t1 t2,
+    access ad m t2 ->
+    access ad m <{t1 = t2}>
 
-  | acc_fun : forall x Tx t ad,
-    (m | t) has_access_to ad ->
-    (m | fn x Tx t) has_access_to ad
+  | acc_fun : forall x Tx t,
+    access ad m t ->
+    access ad m <{fn x Tx t}>
 
-  | acc_call1 : forall t1 t2 ad,
-    (m | t1) has_access_to ad ->
-    (m | call t1 t2) has_access_to ad
+  | acc_call1 : forall t1 t2,
+    access ad m t1 ->
+    access ad m <{call t1 t2}>
 
-  | acc_call2 : forall t1 t2 ad,
-    (m | t2) has_access_to ad ->
-    (m | call t1 t2) has_access_to ad
+  | acc_call2 : forall t1 t2,
+    access ad m t2 ->
+    access ad m <{call t1 t2}>
 
-  | acc_seq1 : forall t1 t2 ad,
-    (m | t1) has_access_to ad ->
-    (m | t1; t2) has_access_to ad
+  | acc_seq1 : forall t1 t2,
+    access ad m t1 ->
+    access ad m <{t1; t2}>
 
-  | acc_seq2 : forall t1 t2 ad,
-    (m | t2) has_access_to ad ->
-    (m | t1; t2) has_access_to ad
-
-  where " '(' m '|' t ')' 'has_access_to' ad " := (access m ad t),
-        " '(' m '/' t ')' 'has_access_to' ad " := (access m ad t).
+  | acc_seq2 : forall t1 t2,
+    access ad m t2 ->
+    access ad m <{t1; t2}>
+  .
 
 (*
   A term has valid accesses if all the addresses it has access to are within
   the bounds of the memory.
 *)
 Definition valid_accesses (m : mem) (t : tm) :=
-  forall ad, (m | t) has_access_to ad -> ad < #m.
+  forall ad, access ad m t -> ad < #m.
 
 (* ------------------------------------------------------------------------- *)
 (* hints                                                                     *)
 (* ------------------------------------------------------------------------- *)
+
+#[export] Hint Unfold valid_accesses  : vac.
 
 #[export] Hint Extern 4 => unfold valid_accesses : vac.
 
@@ -87,17 +81,17 @@ Definition valid_accesses (m : mem) (t : tm) :=
 
 Local Ltac match_acc tactic :=
   match goal with
-  | H : (_ | unit     ) has_access_to _ |- _ => tactic H
-  | H : (_ | N _      ) has_access_to _ |- _ => tactic H
-  | H : (_ | & _ :: _ ) has_access_to _ |- _ => tactic H
-  | H : (_ | new _ _  ) has_access_to _ |- _ => tactic H
-  | H : (_ | * _      ) has_access_to _ |- _ => tactic H
-  | H : (_ | _ = _    ) has_access_to _ |- _ => tactic H
-  | H : (_ | var _    ) has_access_to _ |- _ => tactic H
-  | H : (_ | fn _ _ _ ) has_access_to _ |- _ => tactic H
-  | H : (_ | call _ _ ) has_access_to _ |- _ => tactic H
-  | H : (_ | _ ; _    ) has_access_to _ |- _ => tactic H
-  | H : (_ | spawn _  ) has_access_to _ |- _ => tactic H
+  | H : access _ _ <{unit    }> |- _ => tactic H
+  | H : access _ _ <{N _     }> |- _ => tactic H
+  | H : access _ _ <{& _ :: _}> |- _ => tactic H
+  | H : access _ _ <{new _ _ }> |- _ => tactic H
+  | H : access _ _ <{* _     }> |- _ => tactic H
+  | H : access _ _ <{_ = _   }> |- _ => tactic H
+  | H : access _ _ <{var _   }> |- _ => tactic H
+  | H : access _ _ <{fn _ _ _}> |- _ => tactic H
+  | H : access _ _ <{call _ _}> |- _ => tactic H
+  | H : access _ _ <{_ ; _   }> |- _ => tactic H
+  | H : access _ _ <{spawn _ }> |- _ => tactic H
   end.
 
 Ltac inv_acc := match_acc inv.
@@ -110,51 +104,51 @@ Local Ltac solve_vac_inversion :=
   intros; unfold valid_accesses in *; try split; eauto using access.
 
 Local Lemma inv_vac_ad : forall m ad T,
-  valid_accesses m <{ &ad :: T }> ->
+  valid_accesses m <{&ad :: T}> ->
   valid_accesses m m[ad].tm.
 Proof.
-  intros. intros ad'. destruct (Nat.eq_dec ad ad'); subst; eauto using access.
+  intros. intros ad'. destruct (nat_eq_dec ad ad'); subst; eauto using access.
 Qed.
 
 Local Lemma inv_vac_new : forall m t T,
-  valid_accesses m <{ new T t }> ->
+  valid_accesses m <{new T t}> ->
   valid_accesses m t.
 Proof. solve_vac_inversion. Qed.
 
 Local Lemma inv_vac_load : forall m t,
-  valid_accesses m <{ *t }> ->
+  valid_accesses m <{*t}> ->
   valid_accesses m t.
 Proof. solve_vac_inversion. Qed.
 
 Local Lemma inv_vac_asg : forall m t1 t2,
-  valid_accesses m <{ t1 = t2 }> ->
+  valid_accesses m <{t1 = t2}> ->
   valid_accesses m t1 /\ valid_accesses m t2.
 Proof. solve_vac_inversion. Qed.
 
 Local Lemma inv_vac_fun : forall m x Tx t,
-  valid_accesses m <{ fn x Tx t }> ->
+  valid_accesses m <{fn x Tx t}> ->
   valid_accesses m t.
 Proof. solve_vac_inversion. Qed.
 
 Local Lemma inv_vac_call : forall m t1 t2,
-  valid_accesses m <{ call t1 t2 }> ->
+  valid_accesses m <{call t1 t2}> ->
   valid_accesses m t1 /\ valid_accesses m t2.
 Proof. solve_vac_inversion. Qed.
 
 Local Lemma inv_vac_seq : forall m t1 t2,
-  valid_accesses m <{ t1; t2 }> ->
+  valid_accesses m <{t1; t2}> ->
   valid_accesses m t1 /\ valid_accesses m t2.
 Proof. solve_vac_inversion. Qed.
 
 Ltac inv_vac :=
  match goal with
- | H : valid_accesses _ <{ &_ :: _  }> |- _ => eapply inv_vac_ad   in H as Hvac'
- | H : valid_accesses _ <{ new _ _  }> |- _ => eapply inv_vac_new  in H
- | H : valid_accesses _ <{ * _      }> |- _ => eapply inv_vac_load in H
- | H : valid_accesses _ <{ _ = _    }> |- _ => eapply inv_vac_asg  in H as [? ?]
- | H : valid_accesses _ <{ fn _ _ _ }> |- _ => eapply inv_vac_fun  in H
- | H : valid_accesses _ <{ call _ _ }> |- _ => eapply inv_vac_call in H as [? ?]
- | H : valid_accesses _ <{ _ ; _    }> |- _ => eapply inv_vac_seq  in H as [? ?]
+ | H : valid_accesses _ <{&_ :: _ }> |- _ => eapply inv_vac_ad   in H as Hvac'
+ | H : valid_accesses _ <{new _ _ }> |- _ => eapply inv_vac_new  in H
+ | H : valid_accesses _ <{* _     }> |- _ => eapply inv_vac_load in H
+ | H : valid_accesses _ <{_ = _   }> |- _ => eapply inv_vac_asg  in H as [? ?]
+ | H : valid_accesses _ <{fn _ _ _}> |- _ => eapply inv_vac_fun  in H
+ | H : valid_accesses _ <{call _ _}> |- _ => eapply inv_vac_call in H as [? ?]
+ | H : valid_accesses _ <{_ ; _   }> |- _ => eapply inv_vac_seq  in H as [? ?]
  end.
 
 (* ------------------------------------------------------------------------- *)
@@ -162,26 +156,25 @@ Ltac inv_vac :=
 (* ------------------------------------------------------------------------- *)
 
 Theorem strong_acc_mem : forall m t ad ad',
-  (m | t) has_access_to ad' ->
-  (m | (m[ad'].tm)) has_access_to ad ->
-  (m | t) has_access_to ad.
+  access ad' m t ->
+  access ad  m (m[ad'].tm) ->
+  access ad  m t.
 Proof.
   intros * Hacc ?. induction Hacc; eauto using access;
   match goal with
-  |- (_ | & ?ad' :: _) has_access_to ?ad =>
-    destruct (nat_eq_dec ad ad'); subst
+  |- access ?ad _ <{& ?ad' :: _}> => destruct (nat_eq_dec ad ad'); subst
   end;
   eauto using access.
 Qed.
 
 Lemma acc_dec : forall m t ad,
-  Decidable.decidable ((m | t) has_access_to ad).
+  Decidable.decidable (access ad m t).
 Proof. eauto using classic_decidable. Qed.
 
 (* length ------------------------------------------------------------------ *)
 
 Lemma acc_length : forall m ad ad',
-  (m | (m[ad'].tm)) has_access_to ad ->
+  access ad m (m[ad'].tm) ->
   ad' < #m.
 Proof.
   intros * Hacc. decompose sum (lt_eq_lt_dec ad' (#m)); subst;
@@ -190,35 +183,17 @@ Qed.
 
 Lemma vac_nacc_length : forall m t,
   valid_accesses m t ->
-  ~ ((m | t) has_access_to #m).
+  ~ access (#m) m t.
 Proof.
   intros * Hvac Hacc. specialize (Hvac (#m) Hacc). lia.
 Qed.
-
-(*
-TODO: remove
-
-Lemma vac_length : forall m t ad,
-  valid_accesses m t ->
-  access m t ad ->
-  ad < #m.
-Proof. eauto. Qed.
-
-Corollary vac_neq_length : forall m t ad,
-  valid_accesses m t ->
-  access m t ad ->
-  ad <> #m.
-Proof.
-  intros. eauto using Nat.lt_neq.
-Qed.
-*)
 
 (* ------------------------------------------------------------------------- *)
 (* valid-accesses derives from valid-addresses                               *)
 (* ------------------------------------------------------------------------- *)
 
 Local Lemma acc_then_hasad : forall m t ad,
-  (m | t) has_access_to ad ->
+  access ad m t ->
   t has_address ad \/ (exists ad', m[ad'].tm has_address ad).
 Proof.
   intros * Hacc. induction Hacc; try destruct IHHacc as [? | [? ?]];
@@ -228,7 +203,7 @@ Qed.
 Lemma vad_nacc_length : forall m t,
   forall_memory m (valid_addresses m) ->
   valid_addresses m t ->
-  ~ ((m | t) has_access_to #m).
+  ~ access (#m) m t.
 Proof.
   intros * ? Hvad Hacc. remember (#m) as ad.
   induction Hacc; inversion_vad; eauto. lia.
@@ -261,183 +236,9 @@ Proof.
 Qed.
 
 (* ------------------------------------------------------------------------- *)
-(* properties -- subst                                                       *)
-(* ------------------------------------------------------------------------- *)
-
-Lemma subst_acc : forall m x Tx t t' ad,
-  (m | ([x := t'] t)) has_access_to ad ->
-  (m | call <{ fn x Tx t }> t') has_access_to ad.
-Proof.
-  intros. induction t; eauto using access; simpl in *;
-  try (destruct String.string_dec; eauto using access);
-  inv_clear_acc; auto_specialize; do 2 inv_acc; eauto using access.
-Qed.
-
-(* ------------------------------------------------------------------------- *)
-(* properties -- memory -- add                                               *)
-(* ------------------------------------------------------------------------- *)
-
-(*
-Lemma mem_add_acc : forall m t ad vTr,
-  ~ access m t (#m) ->
-  access (m +++ vTr) t ad ->
-  access m t ad.
-Proof.
-  intros * Hnacc Hacc. remember (m +++ vTr) as m'.
-  induction Hacc; inversion Heqm'; subst; inversion_nacc Hnacc.
-  decompose sum (lt_eq_lt_dec ad' (#m)); subst; try lia;
-  simpl_array; eauto using access. simpl in *. inversion_acc.
-Qed.
-
-Lemma mem_add_nacc : forall m t ad vTr,
-  ~ access m t (#m) ->
-  ~ access m t ad ->
-  ~ access (m +++ vTr) t ad.
-Proof.
-  intros * Hnacc1 Hnacc2 F. induction F; inversion_nacc Hnacc2.
-  decompose sum (lt_eq_lt_dec ad' (#m)); subst; simpl_array;
-  inversion_nacc Hnacc1. eapply IHF; eapply nacc_iff; eauto using not_access.
-Qed.
-*)
-
-(* ------------------------------------------------------------------------- *)
-(* properties -- inheritance                                                 *)
-(* ------------------------------------------------------------------------- *)
-
-(*
-Lemma mem_set_acc : forall m t ad ad' vTr,
-  ~ access m t ad' ->
-  access m[ad' <- vTr] t ad ->
-  access m t ad.
-Proof.
-  intros * Hnacc Hacc.  remember (m[ad' <- vTr]) as m'.
-  induction Hacc; inversion_subst_clear Heqm'; inversion_nacc Hnacc;
-  simpl_array; eauto using access.
-Qed.
-
-Local Lemma mem_set_acc' : forall m t ad ad' v Tr,
-  ~ access m v ad ->
-  access m[ad' <- (v, Tr)] t ad ->
-  access m t ad.
-Proof.
-  intros * Hnacc Hacc. remember (m[ad' <- (v, Tr)]) as m'.
-  induction Hacc; try rename IHHacc into IH;
-  inversion_subst_clear Heqm'; eauto using access.
-  match goal with |- access _ <{ & ?ad :: _ }> _ => rename ad into ad'' end.
-  destruct (Nat.eq_dec ad' ad''); subst;
-  try simpl_array; eauto using access;
-  destruct (Nat.eq_dec ad'' ad); subst; eauto using access.
-  auto_specialize. rewrite (get_set_eq memory_default) in IH. 1: contradiction.
-  eapply not_le. intros Hlen. simpl_array. 
-  eapply Nat.lt_eq_cases in Hlen as [? | ?]; subst;
-  simpl_array; simpl in *; inversion_acc.
-Qed.
-
-Lemma mem_set_nacc1 : forall m t ad ad' vTr,
-  ~ access m t ad' ->
-  ~ access m t ad ->
-  ~ access m[ad' <- vTr] t ad.
-Proof.
-  intros * Hnacc' Hnacc F. remember (m[ad' <- vTr]) as m'.
-  induction F; inversion_nacc Hnacc'; inversion_nacc Hnacc.
-  simpl_array. eauto.
-Qed.
-
-Lemma mem_set_nacc2 : forall m t ad ad' v Tr,
-  ~ access m v ad ->
-  ~ access m t ad ->
-  ~ access m[ad' <- (v, Tr)] t ad.
-Proof.
-  assert (ge_iff_le : forall m n, m >= n <-> n <= m)
-    by (intros; split; destruct n; eauto).
-  assert (forall m ad ad' v,
-    access m[ad' <- v] m[ad' <- v][ad'].tm ad ->
-    ad' < length m). {
-    intros * H. eapply not_ge. rewrite ge_iff_le. intros ?.
-    rewrite (get_set_invalid memory_default) in H; trivial. inversion H.
-  }
-  (* main proof *)
-  intros * ? ? Hacc. remember (m[ad' <- (v, Tr)]) as m'.
-  induction Hacc; inversion_subst_clear Heqm'; eauto using access.
-  match goal with _ : ~ access _ <{ & ?ad :: _ }> _ |- _ => 
-    destruct (Nat.eq_dec ad' ad) as [? | Hneq]; subst;
-    try (assert (ad < #m) by eauto)
-  end;
-  simpl_array; eauto using access.
-Qed.
-*)
-
-(* ------------------------------------------------------------------------- *)
 (* access properties -- inheritance                                          *)
 (* ------------------------------------------------------------------------- *)
 
-Lemma step_none_inherits_access : forall m t t' ad,
-  (m | t') has_access_to ad ->
-  t --[EF_None]--> t' ->
-  (m | t) has_access_to ad.
-Proof.
-  intros. induction_step; try inv_acc; eauto using access, subst_acc.
-Qed.
-
 (*
-Lemma step_alloc_inherits_acc : forall m t t' ad v Tr,
-  valid_accesses m t ->
-  ad <> #m ->
-  access (m +++ (v, Tr)) t' ad ->
-  t --[EF_Alloc (#m) v Tr]--> t' ->
-  access m t ad.
-Proof.
-  intros. induction_step;
-  inversion_vac; inversion_acc; eauto using access; try lia; try simpl_array;
-  eauto using mem_add_acc, vac_nacc_length, access.
-Qed.
-
-Lemma step_read_inherits_acc : forall m t t' ad ad',
-  access m t' ad ->
-  t --[EF_Read ad' m[ad'].tm]--> t' ->
-  access m t ad.
-Proof.
-  intros. induction_step; try inversion_acc; eauto using access.
-  destruct (Nat.eq_dec ad' ad); subst; eauto using access.
-Qed.
-
-Lemma step_write_inherits_acc : forall m t t' ad ad' v Tr,
-  access m[ad' <- (v, Tr)] t' ad ->
-  t --[EF_Write ad' v Tr]--> t' ->
-  access m t ad.
-Proof.
-  intros. induction_step; inversion_acc; eauto using access;
-  destruct (acc_dec m v ad); eauto using mem_set_acc', access;
-  assert (forall t t', t --[EF_Write ad' v Tr]--> t' -> access m t ad)
-    by (intros; induction_step; eauto using access);
-  eauto using access.
-Qed.
-
-Lemma step_spawn_inherits_acc : forall m t t' block ad,
-  access m t' ad ->
-  t --[EF_Spawn block]--> t' ->
-  access m t ad.
-Proof.
-  intros. induction_step; inversion_acc; eauto using access.
-Qed.
-*)
-
-(* ------------------------------------------------------------------------- *)
-(* not-access properties -- preservation                                     *)
-(* ------------------------------------------------------------------------- *)
-
-(*
-
-
-
-Corollary mstep_nacc_preservation : forall m m' t t' ad eff,
-  ad < #m ->
-  valid_accesses m t ->
-  ~ access m t ad ->
-  m / t ==[eff]==> m' / t' ->
-  ~ access m' t' ad.
-Proof.
-Qed.
-
 *)
 
