UnsafeAccess.v
@@ -11,84 +11,81 @@ From Elo Require Import Access.
 From Elo Require Import References.
 
 (* There is a mutable pointer to <ad> in the term. *)
-Inductive UnsafeAccess (m : mem) : tm -> addr -> Prop :=
-  | uacc_mem : forall ad ad' T,
+Inductive unsafe_access (ad : addr) (m : mem) : tm  -> Prop :=
+  | uacc_mem : forall ad' T,
     ad <> ad' ->
-    UnsafeAccess m m[ad'].tm ad ->
-    UnsafeAccess m <{ &ad' :: &T }> ad
+    unsafe_access ad m (m[ad'].tm) ->
+    unsafe_access ad m <{&ad' :: &T}>
 
-  | uacc_ref : forall ad T,
-    UnsafeAccess m <{ &ad :: &T }> ad
+  | uacc_ad : forall T,
+    unsafe_access ad m <{&ad :: &T}>
 
-  | uacc_new : forall T t ad,
-    UnsafeAccess m t ad ->
-    UnsafeAccess m <{ new T t }> ad
+  | uacc_new : forall T t,
+    unsafe_access ad m t ->
+    unsafe_access ad m <{new T t}>
 
-  | uacc_load : forall t ad,
-    UnsafeAccess m t ad ->
-    UnsafeAccess m <{ *t }> ad
+  | uacc_load : forall t,
+    unsafe_access ad m t ->
+    unsafe_access ad m <{*t}>
 
-  | uacc_asg1 : forall t1 t2 ad,
-    UnsafeAccess m t1 ad ->
-    UnsafeAccess m <{ t1 = t2 }> ad
+  | uacc_asg1 : forall t1 t2,
+    unsafe_access ad m t1 ->
+    unsafe_access ad m <{t1 = t2}>
 
-  | uacc_asg2 : forall t1 t2 ad,
-    UnsafeAccess m t2 ad ->
-    UnsafeAccess m <{ t1 = t2 }> ad
+  | uacc_asg2 : forall t1 t2,
+    unsafe_access ad m t2 ->
+    unsafe_access ad m <{t1 = t2}>
 
-  | uacc_fun : forall x Tx t ad,
-    UnsafeAccess m t ad ->
-    UnsafeAccess m <{ fn x Tx t }> ad
+  | uacc_fun : forall x Tx t,
+    unsafe_access ad m t ->
+    unsafe_access ad m <{fn x Tx t}>
 
-  | uacc_call1 : forall t1 t2 ad,
-    UnsafeAccess m t1 ad ->
-    UnsafeAccess m <{ call t1 t2 }> ad
+  | uacc_call1 : forall t1 t2,
+    unsafe_access ad m t1 ->
+    unsafe_access ad m <{call t1 t2}>
 
-  | uacc_call2 : forall t1 t2 ad,
-    UnsafeAccess m t2 ad ->
-    UnsafeAccess m <{ call t1 t2 }> ad
+  | uacc_call2 : forall t1 t2,
+    unsafe_access ad m t2 ->
+    unsafe_access ad m <{call t1 t2}>
 
-  | uacc_seq1 : forall t1 t2 ad,
-    UnsafeAccess m t1 ad ->
-    UnsafeAccess m <{ t1; t2 }> ad
+  | uacc_seq1 : forall t1 t2,
+    unsafe_access ad m t1 ->
+    unsafe_access ad m <{t1; t2}>
 
-  | uacc_seq2 : forall t1 t2 ad,
-    UnsafeAccess m t2 ad ->
-    UnsafeAccess m <{ t1; t2 }> ad
+  | uacc_seq2 : forall t1 t2,
+    unsafe_access ad m t2 ->
+    unsafe_access ad m <{t1; t2}>
   .
 
-Ltac inversion_uacc :=
+(* ------------------------------------------------------------------------- *)
+(* inversion                                                                 *)
+(* ------------------------------------------------------------------------- *)
+
+Local Ltac match_uacc tactic :=
   match goal with
-  | H : UnsafeAccess _ <{ unit     }> _ |- _ => inversion H; subst
-  | H : UnsafeAccess _ <{ N _      }> _ |- _ => inversion H; subst
-  | H : UnsafeAccess _ <{ & _ :: _ }> _ |- _ => inversion H; subst
-  | H : UnsafeAccess _ <{ new _ _  }> _ |- _ => inversion H; subst
-  | H : UnsafeAccess _ <{ * _      }> _ |- _ => inversion H; subst
-  | H : UnsafeAccess _ <{ _ = _    }> _ |- _ => inversion H; subst
-  | H : UnsafeAccess _ <{ var _    }> _ |- _ => inversion H; subst
-  | H : UnsafeAccess _ <{ fn _ _ _ }> _ |- _ => inversion H; subst
-  | H : UnsafeAccess _ <{ call _ _ }> _ |- _ => inversion H; subst
-  | H : UnsafeAccess _ <{ _ ; _    }> _ |- _ => inversion H; subst
-  | H : UnsafeAccess _ <{ spawn _  }> _ |- _ => inversion H; subst
+  | H : unsafe_access _ _ <{unit    }> |- _ => tactic H
+  | H : unsafe_access _ _ <{N _     }> |- _ => tactic H
+  | H : unsafe_access _ _ <{& _ :: _}> |- _ => tactic H
+  | H : unsafe_access _ _ <{new _ _ }> |- _ => tactic H
+  | H : unsafe_access _ _ <{* _     }> |- _ => tactic H
+  | H : unsafe_access _ _ <{_ = _   }> |- _ => tactic H
+  | H : unsafe_access _ _ <{var _   }> |- _ => tactic H
+  | H : unsafe_access _ _ <{fn _ _ _}> |- _ => tactic H
+  | H : unsafe_access _ _ <{call _ _}> |- _ => tactic H
+  | H : unsafe_access _ _ <{_ ; _   }> |- _ => tactic H
+  | H : unsafe_access _ _ <{spawn _ }> |- _ => tactic H
   end.
 
-Ltac inversion_clear_uacc :=
-  match goal with
-  | H : UnsafeAccess _ <{ unit     }> _ |- _ => inversion_subst_clear H
-  | H : UnsafeAccess _ <{ N _      }> _ |- _ => inversion_subst_clear H
-  | H : UnsafeAccess _ <{ & _ :: _ }> _ |- _ => inversion_subst_clear H
-  | H : UnsafeAccess _ <{ new _ _  }> _ |- _ => inversion_subst_clear H
-  | H : UnsafeAccess _ <{ * _      }> _ |- _ => inversion_subst_clear H
-  | H : UnsafeAccess _ <{ _ = _    }> _ |- _ => inversion_subst_clear H
-  | H : UnsafeAccess _ <{ var _    }> _ |- _ => inversion_subst_clear H
-  | H : UnsafeAccess _ <{ fn _ _ _ }> _ |- _ => inversion_subst_clear H
-  | H : UnsafeAccess _ <{ call _ _ }> _ |- _ => inversion_subst_clear H
-  | H : UnsafeAccess _ <{ _ ; _    }> _ |- _ => inversion_subst_clear H
-  | H : UnsafeAccess _ <{ spawn _  }> _ |- _ => inversion_subst_clear H
-  end.
+Ltac inv_uacc := match_uacc inv.
+
+Ltac inv_clear_uacc := match_uacc inv_clear.
+
+(* ------------------------------------------------------------------------- *)
+(* dec                                                                       *)
+(* ------------------------------------------------------------------------- *)
 
 Lemma uacc_dec : forall m t ad,
-  Decidable.decidable (UnsafeAccess m t ad).
+  Decidable.decidable (unsafe_access ad m t).
 Proof. eauto using classic_decidable. Qed.
 
 (* ------------------------------------------------------------------------- *)
@@ -96,92 +93,92 @@ Proof. eauto using classic_decidable. Qed.
 (* ------------------------------------------------------------------------- *)
 
 Local Ltac solve_nuacc :=
-  intros; try (split; intros); eauto using UnsafeAccess.
+  intros; try (split; intros); eauto using unsafe_access.
 
 Lemma nuacc_unit : forall m ad,
-  ~ UnsafeAccess m <{ unit }> ad.
-Proof. intros * ?. inversion_uacc. Qed.
+  ~ unsafe_access ad m <{unit}>.
+Proof. intros * ?. inv_uacc. Qed.
 
 Lemma nuacc_mem : forall m ad ad' T,
   ad <> ad' ->
-  ~ UnsafeAccess m <{ &ad' :: &T }> ad ->
-  ~ UnsafeAccess m m[ad'].tm ad.
+  ~ unsafe_access ad m <{&ad' :: &T}> ->
+  ~ unsafe_access ad m (m[ad'].tm).
 Proof. solve_nuacc. Qed.
 
 Lemma nuacc_new : forall m t ad T,
-  ~ UnsafeAccess m <{ new T t }> ad ->
-  ~ UnsafeAccess m t ad.
+  ~ unsafe_access ad m <{new T t}> ->
+  ~ unsafe_access ad m t.
 Proof. solve_nuacc. Qed.
 
 Lemma nuacc_load : forall m t ad,
-  ~ UnsafeAccess m <{ *t }> ad ->
-  ~ UnsafeAccess m t ad.
+  ~ unsafe_access ad m <{*t}> ->
+  ~ unsafe_access ad m t.
 Proof. solve_nuacc. Qed.
 
 Lemma nuacc_asg : forall m t1 t2 ad,
-  ~ UnsafeAccess m <{ t1 = t2 }> ad ->
-  ~ UnsafeAccess m t1 ad /\ ~ UnsafeAccess m t2 ad.
+  ~ unsafe_access ad m <{t1 = t2}> ->
+  ~ unsafe_access ad m t1 /\ ~ unsafe_access ad m t2.
 Proof. solve_nuacc. Qed.
 
 Lemma nuacc_fun : forall m t ad x Tx,
-  ~ UnsafeAccess m <{ fn x Tx t }> ad ->
-  ~ UnsafeAccess m t ad.
+  ~ unsafe_access ad m <{fn x Tx t}> ->
+  ~ unsafe_access ad m t.
 Proof. solve_nuacc. Qed.
 
 Lemma nuacc_call : forall m t1 t2 ad,
-  ~ UnsafeAccess m <{ call t1 t2 }> ad ->
-  ~ UnsafeAccess m t1 ad /\ ~ UnsafeAccess m t2 ad.
+  ~ unsafe_access ad m <{call t1 t2}> ->
+  ~ unsafe_access ad m t1 /\ ~ unsafe_access ad m t2.
 Proof. solve_nuacc. Qed.
 
 Lemma nuacc_seq : forall m t1 t2 ad,
-  ~ UnsafeAccess m <{ t1; t2 }> ad ->
-  ~ UnsafeAccess m t1 ad /\ ~ UnsafeAccess m t2 ad.
+  ~ unsafe_access ad m <{t1; t2}> ->
+  ~ unsafe_access ad m t1 /\ ~ unsafe_access ad m t2.
 Proof. solve_nuacc. Qed.
 
-Ltac inversion_nuacc :=
+Ltac inv_nuacc :=
   match goal with
-  | H: ~ UnsafeAccess _ <{ & ?ad' :: _ }> ?ad, Hneq : ?ad <> ?ad' |- _ =>
+  | H: ~ unsafe_access _ ?ad <{& ?ad' :: _}>, Hneq : ?ad <> ?ad' |- _ =>
     eapply (nuacc_mem _ _ _ _ Hneq) in H
-  | H: ~ UnsafeAccess _ <{ & ?ad :: & _ }> ?ad |- _ =>
-    contradict H; eauto using UnsafeAccess
-  | H: ~ UnsafeAccess _ <{ new _ _  }> _ |- _ => eapply nuacc_new  in H
-  | H: ~ UnsafeAccess _ <{ * _      }> _ |- _ => eapply nuacc_load in H
-  | H: ~ UnsafeAccess _ <{ _ = _    }> _ |- _ => eapply nuacc_asg  in H as [? ?]
-  | H: ~ UnsafeAccess _ <{ fn _ _ _ }> _ |- _ => eapply nuacc_fun  in H
-  | H: ~ UnsafeAccess _ <{ call _ _ }> _ |- _ => eapply nuacc_call in H as [? ?]
-  | H: ~ UnsafeAccess _ <{ _ ; _    }> _ |- _ => eapply nuacc_seq  in H as [? ?]
+  | H: ~ unsafe_access _ ?ad <{& ?ad :: & _}> |- _ =>
+    contradict H; eauto using unsafe_access
+  | H: ~ unsafe_access _ _ <{new _ _ }> |- _ => eapply nuacc_new  in H
+  | H: ~ unsafe_access _ _ <{* _     }> |- _ => eapply nuacc_load in H
+  | H: ~ unsafe_access _ _ <{_ = _   }> |- _ => eapply nuacc_asg  in H as [? ?]
+  | H: ~ unsafe_access _ _ <{fn _ _ _}> |- _ => eapply nuacc_fun  in H
+  | H: ~ unsafe_access _ _ <{call _ _}> |- _ => eapply nuacc_call in H as [? ?]
+  | H: ~ unsafe_access _ _ <{_ ; _   }> |- _ => eapply nuacc_seq  in H as [? ?]
   end.
 
 (* ------------------------------------------------------------------------- *)
 (* core properties                                                           *)
 (* ------------------------------------------------------------------------- *)
 
-Theorem nuacc_refI : forall m ad v T,
+Theorem nuacc_immutable_reference : forall m ad v T,
   value v ->
-  empty |-- v is (TY_Immut T) ->
-  ~ UnsafeAccess m v ad.
+  empty |-- v is <{{ Immut T }}> ->
+  ~ unsafe_access ad m v.
 Proof.
   intros * Hval ? ?. destruct Hval;
-  inversion_type; inversion_uacc; eauto using UnsafeAccess.
+  inversion_type; inv_uacc; eauto using unsafe_access.
 Qed.
 
-Theorem uacc_soundness : forall m m' t t' ad eff T,
+Theorem uacc_soundness : forall m m' t t' ad e T,
   ad < #m ->
   empty |-- t is T ->
-  ~ UnsafeAccess m t ad ->
-  m / t ==[eff]==> m' / t' ->
+  ~ unsafe_access ad m t ->
+  m / t ==[e]==> m' / t' ->
   m[ad].tm = m'[ad].tm.
 Proof.
   intros. rename ad into ad'. inversion_clear_mstep; trivial.
   - decompose sum (lt_eq_lt_dec ad' (#m)); subst; simpl_array; trivial. lia.
   - decompose sum (lt_eq_lt_dec ad' ad); subst; simpl_array; trivial.
-    generalize dependent T. induction_step; intros;
-    inversion_nuacc; inversion_type; eauto using UnsafeAccess.
-    inversion_type. exfalso. eauto using UnsafeAccess.
+    generalize dependent T.
+    induction_step; intros; inversion_type; inv_nuacc; eauto.
+    inversion_type. exfalso. eauto using unsafe_access.
 Qed.
 
 Lemma uacc_then_acc : forall m t ad,
-  UnsafeAccess m t ad ->
+  unsafe_access ad m t ->
   access m t ad.
 Proof.
   intros * Huacc. induction Huacc; eauto using access.
@@ -189,7 +186,7 @@ Qed.
 
 Lemma nacc_then_nuacc : forall m t ad,
   ~ access m t ad ->
-  ~ UnsafeAccess m t ad.
+  ~ unsafe_access m t ad.
 Proof.
   intros * ? Huacc. induction Huacc; eauto using access.
 Qed.
@@ -197,11 +194,11 @@ Qed.
 Lemma step_write_requires_uacc : forall m t t' ad v Tr T,
   empty |-- t is T ->
   t --[EF_Write ad v Tr]--> t' ->
-  UnsafeAccess m t ad.
+  unsafe_access m t ad.
 Proof.
   intros. generalize dependent T.
-  induction_step; intros * ?; inversion_type; eauto using UnsafeAccess.
-  inversion_type. eauto using UnsafeAccess.
+  induction_step; intros * ?; inversion_type; eauto using unsafe_access.
+  inversion_type. eauto using unsafe_access.
 Qed.
 
 (* ------------------------------------------------------------------------- *)
@@ -209,79 +206,79 @@ Qed.
 (* ------------------------------------------------------------------------- *)
 
 Local Lemma subst_nuacc' : forall m t ad v x,
-  ~ UnsafeAccess m v ad ->
-  ~ UnsafeAccess m t ad ->
-  ~ UnsafeAccess m ([x := v] t) ad.
+  ~ unsafe_access ad m v ->
+  ~ unsafe_access ad m t ->
+  ~ unsafe_access m ([x := v] t) ad.
 Proof.
   intros. intros ?. induction t; eauto; simpl in *;
   try (destruct String.string_dec; eauto);
-  inversion_uacc; inversion_nuacc; eauto.
+  inv_uacc; inv_nuacc; eauto.
 Qed.
 
 Local Corollary subst_nuacc : forall m t ad v x Tx,
-  ~ UnsafeAccess m v ad ->
-  ~ UnsafeAccess m <{ fn x Tx t }> ad ->
-  ~ UnsafeAccess m ([x := v] t) ad.
+  ~ unsafe_access ad m v ->
+  ~ unsafe_access ad m <{fn x Tx t}> ->
+  ~ unsafe_access m ([x := v] t) ad.
 Proof.
-  intros. inversion_nuacc. eauto using subst_nuacc'.
+  intros. inv_nuacc. eauto using subst_nuacc'.
 Qed.
 
 Lemma mem_add_uacc : forall m t ad vTr,
   ~ access m t (#m) ->
-  UnsafeAccess (m +++ vTr) t ad ->
-  UnsafeAccess m t ad.
+  unsafe_access ad (m +++ vTr) t ->
+  unsafe_access m t ad.
 Proof.
   intros * Hnacc Huacc. remember (m +++ vTr) as m'.
   induction Huacc; inversion Heqm'; subst; inversion_nacc Hnacc;
-  eauto using UnsafeAccess.
+  eauto using unsafe_access.
   eapply uacc_mem; trivial.
   decompose sum (lt_eq_lt_dec ad' (#m)); subst; simpl_array; eauto; lia.
 Qed.
 
 Local Lemma mem_add_nuacc : forall m t ad vTr,
-  ~ UnsafeAccess m t (#m) ->
-  ~ UnsafeAccess m t ad ->
-  ~ UnsafeAccess (m +++ vTr) t ad.
+  ~ unsafe_access (#m) m t ->
+  ~ unsafe_access ad m t ->
+  ~ unsafe_access (m +++ vTr) t ad.
 Proof.
   intros. intros Huacc.
-  induction Huacc; eauto using UnsafeAccess; inversion_nuacc;
-  eauto using UnsafeAccess.
+  induction Huacc; eauto using unsafe_access; inv_nuacc;
+  eauto using unsafe_access.
   decompose sum (lt_eq_lt_dec ad' (#m)); subst; simpl_array;
-  simpl in *; try inversion_uacc; eauto using UnsafeAccess.
+  simpl in *; try inv_uacc; eauto using unsafe_access.
   assert (#m <> ad') by eauto using Nat.lt_neq, Nat.neq_sym.
-  inversion_nuacc. eauto.
+  inv_nuacc. eauto.
 Qed.
 
 Lemma mem_set_uacc : forall m t ad ad' vTr,
   ~ access m t ad' ->
-  UnsafeAccess m[ad' <- vTr] t ad ->
-  UnsafeAccess m t ad.
+  unsafe_access ad m[ad' <- vTr] t ->
+  unsafe_access m t ad.
 Proof.
   intros * Hnacc Huacc. remember (m[ad' <- vTr]) as m'.
   induction Huacc; inversion_subst_clear Heqm'; inversion_nacc Hnacc;
-  eauto using UnsafeAccess. simpl_array. eauto using UnsafeAccess.
+  eauto using unsafe_access. simpl_array. eauto using unsafe_access.
 Qed.
 
 Local Lemma mem_set_nuacc : forall m t ad ad' v Tr,
-  ~ UnsafeAccess m v ad ->
-  ~ UnsafeAccess m t ad ->
-  ~ UnsafeAccess m[ad' <- (v, Tr)] t ad.
+  ~ unsafe_access ad m v ->
+  ~ unsafe_access ad m t ->
+  ~ unsafe_access m[ad' <- (v, Tr)] t ad.
 Proof.
   assert (ge_iff_le : forall m n, m >= n <-> n <= m)
     by (intros; split; destruct n; eauto).
   assert (Hlen : forall m ad ad' v Tr,
-    UnsafeAccess m[ad' <- (v, Tr)] m[ad' <- (v, Tr)][ad'].tm ad ->
+    unsafe_access ad m[ad' <- (v, Tr)] m[ad' <- (v, Tr)][ad'].tm ->
     ad' < #m). {
     intros * H. eapply not_ge. rewrite ge_iff_le. intros ?.
     rewrite (get_set_invalid memory_default) in H; trivial. inversion H.
   }
   (* main proof *)
   intros * ? ? Huacc. remember (m[ad' <- (v, Tr)]) as m'.
-  induction Huacc; inversion_subst_clear Heqm'; eauto using UnsafeAccess.
+  induction Huacc; inversion_subst_clear Heqm'; eauto using unsafe_access.
   match goal with _ : _ <> ?ad |- _ => rename ad into ad'' end. 
   destruct (Nat.eq_dec ad' ad'') as [? | Hneq]; subst;
   try (assert (ad'' < #m) by eauto using Hlen);
-  simpl_array; eauto using UnsafeAccess.
+  simpl_array; eauto using unsafe_access.
 Qed.
 
 (* ------------------------------------------------------------------------- *)
@@ -298,35 +295,35 @@ Proof.
 Qed.
 
 Local Lemma contains_nuacc : forall m t t' ad,
-  ~ UnsafeAccess m t ad ->
+  ~ unsafe_access ad m t ->
   t contains t' ->
-  ~ UnsafeAccess m t' ad.
+  ~ unsafe_access m t' ad.
 Proof.
-  intros * ? Hcon ?. induction Hcon; subst; eauto; inversion_nuacc; eauto.
+  intros * ? Hcon ?. induction Hcon; subst; eauto; inv_nuacc; eauto.
 Qed.
 
 Lemma step_none_nuacc_preservation : forall m t t' ad,
-  ~ UnsafeAccess m t ad ->
+  ~ unsafe_access ad m t ->
   t --[EF_None]--> t' ->
-  ~ UnsafeAccess m t' ad.
+  ~ unsafe_access m t' ad.
 Proof.
   intros. intros F. induction_step;
-  inversion_nuacc; try contradiction;
-  try inversion_clear_uacc; eauto using UnsafeAccess.
+  inv_nuacc; try contradiction;
+  try inversion_clear_uacc; eauto using unsafe_access.
   contradict F. eauto using subst_nuacc.
 Qed.
 
 Lemma step_alloc_nuacc_preservation : forall m t t' ad v Tr,
   ad <> #m ->
   valid_accesses m t ->
-  ~ UnsafeAccess m t ad ->
+  ~ unsafe_access ad m t ->
   t --[EF_Alloc (#m) v Tr]--> t' ->
-  ~ UnsafeAccess (m +++ (v, Tr)) t' ad.
+  ~ unsafe_access (m +++ (v, Tr)) t' ad.
 Proof.
   intros. intros ?. induction_step;
-  inversion_vac; inversion_nuacc; inversion_uacc;
-  eauto using UnsafeAccess; try simpl_array;
-  match goal with F : UnsafeAccess (_ +++ _) _ _ |- _ => contradict F end;
+  inversion_vac; inv_nuacc; inv_uacc;
+  eauto using unsafe_access; try simpl_array;
+  match goal with F : unsafe_access (_ +++ _) _ _ |- _ => contradict F end;
   eauto using mem_add_nuacc, vac_nacc_length, nacc_then_nuacc.
 Qed.
 
@@ -334,37 +331,37 @@ Lemma step_read_nuacc_preservation : forall m t t' ad ad' T,
   forall_memory m value ->
   empty |-- t is T ->
   consistently_typed_references m t ->
-  ~ UnsafeAccess m t ad ->
+  ~ unsafe_access ad m t ->
   t --[EF_Read ad' m[ad'].tm]--> t' ->
-  ~ UnsafeAccess m t' ad.
+  ~ unsafe_access m t' ad.
 Proof.
   intros * Hval. intros. intros ?. generalize dependent T.
   induction_step; intros;
-  inversion_ctr; inversion_type; inversion_nuacc; try inversion_clear_uacc;
+  inversion_ctr; inversion_type; inv_nuacc; try inversion_clear_uacc;
   eauto; inversion_type; destruct (Nat.eq_dec ad' ad); subst;
-  eauto using UnsafeAccess; inversion_ctr;
-  match goal with F : UnsafeAccess _ _[_].tm _ |- _ => contradict F end;
+  eauto using unsafe_access; inversion_ctr;
+  match goal with F : unsafe_access _ _[_].tm _ |- _ => contradict F end;
   eauto using nuacc_refI.
 Qed.
 
 Lemma step_write_nuacc_preservation : forall m t t' ad ad' v Tr,
-  ~ UnsafeAccess m t ad ->
+  ~ unsafe_access ad m t ->
   t --[EF_Write ad' v Tr]--> t' ->
-  ~ UnsafeAccess m[ad' <- (v, Tr)] t' ad.
+  ~ unsafe_access m[ad' <- (v, Tr)] t' ad.
 Proof.
   intros. intros ?. induction_step;
-  inversion_nuacc; inversion_clear_uacc; eauto using UnsafeAccess;
-  match goal with H : UnsafeAccess _ ?t _ |- _ => rename t into tx end;
+  inv_nuacc; inversion_clear_uacc; eauto using unsafe_access;
+  match goal with H : unsafe_access _ ?t _ |- _ => rename t into tx end;
   eapply (mem_set_nuacc _ tx _ _ v);
   eauto using step_write_contains, contains_nuacc.
 Qed.
 
 Lemma step_spawn_nuacc_preservation : forall m t t' ad block,
-  ~ UnsafeAccess m t ad ->
+  ~ unsafe_access ad m t ->
   t --[EF_Spawn block]--> t' ->
-  ~ UnsafeAccess m t' ad.
+  ~ unsafe_access m t' ad.
 Proof.
-  intros. intros ?. induction_step; try inversion_nuacc; inversion_uacc; eauto.
+  intros. intros ?. induction_step; try inv_nuacc; inv_uacc; eauto.
 Qed.
 
 (* ------------------------------------------------------------------------- *)
@@ -372,10 +369,10 @@ Qed.
 (* ------------------------------------------------------------------------- *)
 
 Lemma step_spawn_uacc_inheritance : forall m t t' ad block,
-  UnsafeAccess m t' ad ->
+  unsafe_access ad m t' ->
   t --[EF_Spawn block]--> t' ->
-  UnsafeAccess m t ad.
+  unsafe_access m t ad.
 Proof.
-  intros. induction_step; inversion_uacc; eauto using UnsafeAccess.
+  intros. induction_step; inv_uacc; eauto using unsafe_access.
 Qed.
 
