AccessExt.v
@@ -1,4 +1,5 @@
 From Coq Require Import Arith.Arith.
+From Coq Require Import Lia.
 
 From Elo Require Import Util.
 From Elo Require Import Array.
@@ -9,203 +10,106 @@ From Elo Require Import Access.
 From Elo Require Import NotAccess.
 
 (* ------------------------------------------------------------------------- *)
-(* preservation                                                              *)
+(* inheritance                                                               *)
 (* ------------------------------------------------------------------------- *)
 
-Local Lemma nacc_subst_preservation : forall m t tx ad x,
-  ~ access m t ad ->
-  ~ access m tx ad ->
-  ~ access m ([x := tx] t) ad.
+Local Lemma acc_subst_inheritance : forall m x Tx t t' ad,
+  access ad m ([x := t'] t) ->
+  access ad m <{call <{fn x Tx t}> t'}>.
 Proof.
-  intros * Hnacc ?. generalize dependent tx.
-  induction t; intros; trivial; simpl;
-  try solve [eapply nacc_iff; inv_nacc Hnacc; eauto using not_access];
-  destruct string_eq_dec; trivial.
-  inv_nacc Hnacc. eapply nacc_iff. eauto using not_access.
+  intros. induction t; eauto using access; simpl in *;
+  try (destruct string_eq_dec; eauto using access);
+  inv_clear_acc; auto_specialize; do 2 inv_acc; eauto using access.
 Qed.
 
-Local Lemma nacc_mem_add_preservation : forall m t ad vT,
-  ~ access m t (#m) ->
-  ~ access m t ad ->
-  ~ access (m +++ vT) t ad.
+Local Lemma acc_mem_add_inheritance : forall m t ad vT,
+  ~ access (#m) m t ->
+  access ad (m +++ vT) t ->
+  access ad m t.
 Proof.
-  intros * Hnacc1 Hnacc2 F. induction F; inv_nacc Hnacc2.
-  decompose sum (lt_eq_lt_dec ad' (#m)); subst; simpl_array; inv_nacc Hnacc1.
-  eapply IHF; trivial. eapply nacc_iff. eauto using not_access.
+  intros * Hnacc Hacc. remember (m +++ vT) as m'.
+  induction Hacc; inv Heqm'; inv_nacc Hnacc.
+  decompose sum (lt_eq_lt_dec ad' (#m)); subst; try lia;
+  simpl_array; eauto using access. simpl in *. inv_acc.
 Qed.
 
-Local Lemma nacc_mem_set_preservation : forall m t ad ad' v T,
-  ~ access m v ad ->
-  ~ access m t ad ->
-  ~ access m[ad' <- (v, T)] t ad.
+Local Lemma acc_mem_set_inheritance : forall m t ad ad' v T,
+  ~ access ad m v ->
+  access ad m[ad' <- (v, T)] t ->
+  access ad m t.
 Proof.
-  assert (ge_iff_le : forall m n, m >= n <-> n <= m)
-    by (intros; split; destruct n; eauto).
-  assert (forall m ad ad' v,
-    access m[ad' <- v] m[ad' <- v][ad'].tm ad -> ad' < length m). {
-      intros * H. eapply not_ge. rewrite ge_iff_le. intros ?.
-      rewrite (get_set_invalid memory_default) in H; trivial. inversion H.
-  }
-  (* main proof *)
-  intros * ? ? Hacc. remember (m[ad' <- (v, T)]) as m'.
-  induction Hacc; inv_clear Heqm'; eauto using access.
-  match goal with
-  | _ : ~ access _ <{ & ?ad :: _ }> _ |- _ => 
-    decompose sum (nat_eq_dec ad' ad); subst; try (assert (ad < #m) by eauto)
-  end;
-  simpl_array; eauto using access.
+  intros * Hnacc Hacc. remember (m[ad' <- (v, T)]) as m'.
+  induction Hacc; inv Heqm'; eauto using access.
+  match goal with |- access _ _ <{& ?ad :: _}> => rename ad into ad'' end.
+  destruct (nat_eq_dec ad' ad''); subst; try (simpl_array; eauto using access);
+  destruct (nat_eq_dec ad'' ad); subst; eauto using access.
+  rewrite (get_set_eq memory_default) in IHHacc. 1: contradiction.
+  eapply not_le. intros Hlen. simpl_array. 
+  eapply Nat.lt_eq_cases in Hlen as [? | ?]; subst;
+  simpl_array; simpl in *; inv_acc.
 Qed.
 
-(* ------------------------------------------------------------------------- *)
+(* alternative for mem_set ------------------------------------------------- *)
 
-Local Lemma nacc_tstep_none_preservation : forall m t t' ad,
-  ~ access m t ad ->
+Local Lemma alt_acc_mem_set_inheritance : forall m t ad ad' vT,
+  ~ access ad' m t ->
+  access ad m[ad' <- vT] t ->
+  access ad m t.
+Proof.
+  intros * Hnacc Hacc. remember (m[ad' <- vT]) as m'.
+  induction Hacc; inv_clear Heqm'; inv_nacc Hnacc; simpl_array;
+  eauto using access.
+Qed.
+
+(* tstep ------------------------------------------------------------------- *)
+
+Local Lemma acc_tstep_none_inheritance  : forall m t t' ad,
+  access ad m t' ->
   t --[EF_None]--> t' ->
-  ~ access m t' ad.
+  access ad m t.
 Proof.
-  intros * Hnacc. intros. induction_step; inv_nacc Hnacc;
-  try solve [eapply nacc_iff; eauto using not_access].
-  match goal with H : ~ access _ <{ fn _ _ _ }> _ |- _ => inv_nacc H end.
-  eauto using nacc_subst_preservation.
+  intros. induction_step; try inv_acc;
+  eauto using access, acc_subst_inheritance .
 Qed.
 
-Local Lemma nacc_tstep_alloc_preservation : forall m t t' ad v T,
+Local Lemma acc_tstep_alloc_inheritance : forall m t t' ad v T,
   ad < #m ->
   forall_memory m (valid_addresses m) ->
-  valid_addresses m t ->
-  ~ access m t ad ->
+  valid_addresses m t' ->
+  access ad (m +++ (v, T)) t' ->
   t --[EF_Alloc (#m) v T]--> t' ->
-  ~ access (m +++ (v, T)) t' ad.
+  access ad m t.
 Proof.
-  intros * ? ? ? Hnacc ?.
-  induction_step; inversion_vad; inv_nacc Hnacc; eapply nacc_iff;
-  eauto using not_access, nacc_mem_add_preservation, vad_nacc_length.
-  eapply nacc_ad. eauto using not_eq_sym, Nat.lt_neq.
-  simpl_array. eauto using nacc_mem_add_preservation, vad_nacc_length.
+  intros. induction_step; inversion_vad; inv_acc; eauto; try lia;
+  try simpl_array; eauto using access, vad_nacc_length, acc_mem_add_inheritance.
 Qed.
 
-Local Lemma nacc_tstep_read_preservation : forall m t t' ad ad',
-  ~ access m t ad ->
+Local Lemma acc_tstep_read_inheritance : forall m t t' ad ad',
+  access ad m t' ->
   t --[EF_Read ad' m[ad'].tm]--> t' ->
-  ~ access m t' ad.
+  access ad m t.
 Proof.
-  intros * Hnacc ?. induction_step; inv_nacc Hnacc;
-  try solve [eapply nacc_iff; eauto using not_access].
-  match goal with H : ~ access _ _ _ |- _ => inv_nacc H end.
+  intros. induction_step; try inv_acc; eauto using access.
+  destruct (nat_eq_dec ad' ad); subst; eauto using access.
 Qed.
 
-Local Lemma nacc_tstep_write_preservation : forall m t t' ad ad' v T,
-  ~ access m t ad ->
+Local Lemma acc_tstep_write_inheritance : forall m t t' ad ad' v T,
+  access ad m[ad' <- (v, T)] t' ->
   t --[EF_Write ad' v T]--> t' ->
-  ~ access m[ad' <- (v, T)] t' ad.
+  access ad m t.
 Proof.
-  assert (forall m t t' ad ad' v T,
-    ~ access m t ad ->
-    t --[EF_Write ad' v T]--> t' ->
-    ~ access m v ad)
-    by (intros; induction_step; eauto using access).
-  (* main proof *)
-  intros * Hnacc ?. induction_step; inv_nacc Hnacc;
-  eapply nacc_iff; eauto using not_access, nacc_mem_set_preservation.
+  intros. induction_step; inv_acc; eauto using access;
+  destruct (acc_dec m v ad); eauto using access, acc_mem_set_inheritance;
+  assert (forall t t', t --[EF_Write ad' v T]--> t' -> access ad m t)
+    by (intros; induction_step; eauto using access);
+  eauto using access.
 Qed.
 
-Local Lemma nacc_tstep_spawn_preservation : forall m t t' block ad,
-  ~ access m t ad ->
+Local Lemma acc_tstep_spawn_inheritance : forall m t t' block ad,
+  access ad m t' ->
   t --[EF_Spawn block]--> t' ->
-  ~ access m t' ad.
+  access ad m t.
 Proof.
-  intros * Hnacc ?. induction_step; inv_nacc Hnacc;
-  eapply nacc_iff; eauto using not_access.
-Qed.
-
-Local Corollary nacc_mstep_preservation : forall m m' t t' e ad,
-  ad < #m ->
-  forall_memory m (valid_addresses m) ->
-  valid_addresses m t ->
-  ~ access m t ad ->
-  m / t ==[e]==> m' / t' ->
-  ~ access m' t' ad.
-Proof.
-  intros. inversion_mstep;
-  eauto using nacc_tstep_none_preservation,
-    nacc_tstep_alloc_preservation,
-    nacc_tstep_read_preservation,
-    nacc_tstep_write_preservation.
-Qed.
-
-(* ------------------------------------------------------------------------- *)
-
-Local Lemma nacc_thread_default_preservation : forall m ad,
-  ~ access m thread_default ad.
-Proof.
-  intros. eapply nacc_iff. eauto using not_access.
-Qed.
-
-Local Lemma nacc_spawn_block_preservation : forall m t t' block ad,
-  ~ access m t ad ->
-  t --[EF_Spawn block]--> t' ->
-  ~ access m block ad.
-Proof.
-Abort.
-
-Local Lemma nacc_untouched_threads_preservation :
-  forall m m' ths tid tid' t' e ad,
-    forall_threads ths (fun t => ~ access m t ad) ->
-    tid <> tid' ->
-    tid' < #ths ->
-    m / ths[tid] ==[e]==> m' / t' ->
-    ~ access m' ths[tid'] ad.
-Proof.
-Abort.
-
-Corollary nacc_cstep_preservation : forall m m' ths ths' tid e,
-  forall_memory m (~ access m) ->
-  forall_threads ths (~ access m) ->
-  m / ths ~~[tid, e]~~> m' / ths' ->
-  forall_threads ths' (~ access m').
-Proof.
-Abort.
-
-(* ------------------------------------------------------------------------- *)
-
-Local Lemma nacc_tstep_alloc_mem_preservation : forall m t t' v T,
-  ~ access m t ->
-  forall_memory m (~ access m) ->
-  t --[EF_Alloc (#m) v T]--> t' ->
-  forall_memory  (m +++ (v, T)) (~ access (m +++ (v, T))).
-Proof.
-Qed.
-
-Local Lemma nacc_tstep_write_mem_preservation : forall m t t' ad v T,
-  ~ access m t ->
-  forall_memory m (~ access m) ->
-  t --[EF_Write ad v T]--> t' ->
-  forall_memory m[ad <- (v, T)] (~ access m[ad <- (v, T)]).
-Proof.
-Qed.
-
-Local Corollary nacc_mstep_mem_preservation : forall m m' t t' e,
-  ~ access m t ->
-  forall_memory m (~ access m) ->
-  m / t ==[e]==> m' / t' ->
-  forall_memory m' (~ access m').
-Proof.
-Qed.
-
-Local Corollary nacc_cstep_mem_preservation : forall m m' ths ths' tid e,
-  forall_threads ths (~ access m) ->
-  forall_memory m (~ access m) ->
-  m / ths ~~[tid, e]~~> m' / ths' ->
-  forall_memory m' (~ access m').
-Proof.
-Qed.
-
-(* ------------------------------------------------------------------------- *)
-
-Theorem not_access_preservation : forall m m' ths ths' tid e,
-  forall_program m ths (~ access m) ->
-  m / ths ~~[tid, e]~~> m' / ths' ->
-  forall_program m' ths' (~ access m').
-Proof.
+  intros. induction_step; inv_acc; eauto using access.
 Qed.
 
